ulib/FStar.Reflection.Types.fsti
@@ -4,4 +4,3 @@ assume new type binder
 assume new type term
 assume new type env
 assume new type fv
-assume new type bv
